STLC_SuccNat/Lifted_Norm.v
@@ -32,7 +32,20 @@ Inductive appears_free_in' : string -> tm' -> Prop :=
     y <> x -> appears_free_in' x t12' ->
       appears_free_in' x (abs' y T11' t12')
   (* nats*)
-  |afi_succ' : forall x t1', appears_free_in' x t1' -> appears_free_in' x (succ' t1').
+  |afi_succ' : forall x t1', appears_free_in' x t1' -> appears_free_in' x (succ' t1')
+  (* lists *)
+  |afi_cons1' : forall x t1' t2', appears_free_in' x t1' -> appears_free_in' x (cons' t1' t2')
+  |afi_cons2' : forall x t1' t2', appears_free_in' x t2' -> appears_free_in' x (cons' t1' t2')
+  
+  |afi_case1' : forall x y z t1' tnil' tcons',
+    appears_free_in' x t1' -> appears_free_in' x (case' t1' tnil' y z tcons')
+  |afi_case2' : forall x y z t1' tnil' tcons',
+    appears_free_in' x tnil' -> appears_free_in' x (case' t1' tnil' y z tcons')
+  |afi_case3' : forall x y z t1' tnil' tcons',
+    y <> x ->
+    z <> x ->
+    appears_free_in' x tcons' ->
+      appears_free_in' x (case' t1' tnil' y z tcons').
 
 Hint Constructors appears_free_in' : core.
 
@@ -60,13 +73,27 @@ Proof.
     + rewrite update_neq; [| assumption].
       rewrite update_neq; [| assumption].
       auto.
+  - (* T_Case' *)
+    apply T_Case';
+      [ apply IHhas_type'1 |
+        apply IHhas_type'2 |
+        apply IHhas_type'3 ];
+      intros x1 Hafi;
+      try apply H2; auto.
+    destruct (eqb_spec x x1);
+    destruct (eqb_spec y x1); subst.
+    + repeat rewrite update_eq. auto.
+    + repeat rewrite update_eq. auto.
+    + repeat (rewrite update_neq; auto;
+      rewrite update_eq).
+    + repeat (rewrite update_neq; auto).
 Qed.
 
-Theorem false_eqb_string : forall x y : string,
-   x <> y -> String.eqb x y = false.
-Proof.
-  intros x y. rewrite String.eqb_neq.
-  intros H. apply H. Qed.
+Ltac false_eqb_string :=
+  try match goal with
+      | [ H: (?x <> ?y)%string |- _ ] => apply eqb_neq in H; rewrite H in *
+      | [ H: ?x <> ?y |- _ ] => apply eqb_neq in H; rewrite H in *
+  end.
 
 Lemma free_in_context' : forall x t' T' Gamma',
    appears_free_in' x t' ->
@@ -78,7 +105,11 @@ Proof with eauto.
   - (* T_Abs' *)
     destruct IHHtyp as [T' Hctx]... exists T'.
     unfold update, t_update in Hctx.
-    rewrite false_eqb_string in Hctx...
+    false_eqb_string...
+  - (* T_Case' *)
+    destruct IHHtyp3 as [T1' Hctx]... exists T1'.
+    unfold update, t_update in Hctx.
+    repeat false_eqb_string...
 Qed.
 
 Corollary typable_empty__closed' : forall t' T',
@@ -94,6 +125,7 @@ Fixpoint R' (T':ty') (t':tm') : Prop :=
   (match T' with
     | Nat' => True
     | Arrow' T1' T2' => (forall s', R' T1' s' -> R' T2' (app' t' s'))
+    | NatList' => True
     end).
 
 Lemma R'_halts' : forall {T'} {t'}, R' T' t' -> halts' t'.
@@ -139,6 +171,10 @@ Proof.
   split. eapply preservation'; eauto.
   split. apply (step'_preserves_halting _ _ E); eauto.
   auto.
+  (* NatList *)
+  split. eapply preservation'; eauto.
+  split. apply (step'_preserves_halting _ _ E); eauto.
+  auto.
 Qed.
 
 Lemma multistep'_preserves_R' : forall T' t' t1',
@@ -164,6 +200,10 @@ Proof.
   eapply ST_App1'. apply E.
   apply RRt; auto.
   (* Nat *)
+  split. auto.
+  split. apply (step'_preserves_halting _ _ E); eauto.
+  auto.
+  (* NatList *)
   split. auto.
   split. apply (step'_preserves_halting _ _ E); eauto.
   auto.
@@ -202,6 +242,13 @@ Proof with eauto.
     intros H; eauto.
    - (* Succ' *)
     rewrite IHt'...
+  - (* Cons' *)
+    rewrite IHt'1, IHt'2...
+  - (* Case' *)
+    rewrite IHt'1, IHt'2...
+    destruct (eqb_spec x s); simpl...
+    destruct (eqb_spec x s0); simpl...
+    rewrite IHt'3...
 Qed.
 
 Lemma subst'_closed': forall t',
@@ -219,7 +266,7 @@ Qed.
 
 Fixpoint closed'_env' (env':env') :=
   match env' with
-  | nil => True
+  | [] => True
   | (x,t')::env1' => closed' t' /\ closed'_env' env1'
   end.
 
@@ -241,6 +288,14 @@ Proof with eauto.  (* rather slow this way *)
      inversion A.
     - (* succ' *)
      inversion A; subst...
+    - (* nil' *)
+     inversion A; subst...
+    - (* cons' *)
+     inversion A; subst...
+    - (* case' *)
+     destruct (eqb_spec x s);
+     destruct (eqb_spec x s0);
+     eauto; inversion A; subst...
 Qed.
 
 Lemma duplicate_subst' : forall t1' x t' v',
@@ -260,13 +315,13 @@ Proof with eauto.
    + subst. exfalso...
    + subst. simpl. rewrite String.eqb_refl. apply subst'_closed'...
    + subst. simpl. rewrite String.eqb_refl. rewrite subst'_closed'...
-   + simpl. rewrite false_eqb_string... rewrite false_eqb_string...
+   + simpl. repeat false_eqb_string...
   - (* abs' *)
    destruct (eqb_spec x s); destruct (eqb_spec x1 s).
    + subst. exfalso...
-   + subst. simpl. rewrite eqb_refl. rewrite false_eqb_string...
-   + subst. simpl. rewrite eqb_refl. rewrite false_eqb_string...
-   + simpl. rewrite false_eqb_string... rewrite false_eqb_string...
+   + subst. simpl. rewrite eqb_refl. false_eqb_string...
+   + subst. simpl. rewrite eqb_refl. false_eqb_string...
+   + simpl. repeat false_eqb_string...
      rewrite IHt'...
   - (* app' *)
    rewrite IHt'1, IHt'2...
@@ -274,6 +329,19 @@ Proof with eauto.
    reflexivity.
   - (* succ' *)
    rewrite IHt'...
+  - (* nil' *)
+   reflexivity.
+  - (* cons' *)
+   rewrite IHt'1, IHt'2...
+  - (* case' *)
+   destruct (eqb_spec x1 s); simpl;
+   destruct (eqb_spec x s);
+   simpl; subst;
+     try rewrite IHt'1, IHt'2...
+   + destruct (eqb_spec x1 s0);
+     destruct (eqb_spec x s0);
+     subst;
+     try rewrite IHt'1, IHt'2, IHt'3...
 Qed.
 
 Lemma subst'_msubst': forall env' x v' t', closed' v' -> closed'_env' env' ->
@@ -288,7 +356,7 @@ Proof.
 Qed.
 
 Inductive instantiation' : tass' -> env' -> Prop :=
-  | V_nil' : instantiation' nil nil
+  | V_nil' : instantiation' [] []
   | V_cons' : forall x T' v' c e,
       value' v' -> R' T' v' ->
       instantiation' c e ->
@@ -396,7 +464,7 @@ Proof.
           + auto.
           + rewrite H.
             clear - c n. induction c.
-            simpl.  rewrite false_eqb_string; auto.
+            simpl. false_eqb_string; auto.
             simpl. destruct a.  unfold update, t_update.
             destruct (String.eqb s x0); auto. }
         unfold R'. fold R'. split.
@@ -408,7 +476,7 @@ Proof.
          apply multistep'_preserves_R1' with (msubst' ((x,v)::env0') t').
             eapply T_App'. eauto.
             apply R'_typable_empty; auto.
-            eapply multi_step'_trans. eapply multistep'_App2'; eauto.
+            eapply multi_step'_trans. eapply multistep'_app2'; eauto.
             eapply multi_step with (y:= (msubst' ((x, v) :: env0') t')); [|apply multi_refl].
             simpl.  rewrite subst'_msubst'.
             eapply ST_AppAbs'; eauto.
@@ -441,14 +509,101 @@ Proof.
       apply (canonical_forms_nat' v A) in Hv as [n Hv].
       rewrite Hv. exists (const' (map (fun '(n0,pc) => (S (n0),pc)) n)); eauto.
       auto.
+  - (* T_Nil' *)
+    rewrite msubst'_nil'.
+    split. auto. split. apply value'_halts'; auto. auto.
+  - (* T_Cons' *)
+    rewrite msubst'_cons'.
+    pose proof (IHHT1 c H env0' V) as P1.
+    pose proof (IHHT2 c H env0' V) as P2.
+    split. apply T_Cons'.
+    destruct P1 as [HT _]. auto.
+    destruct P2 as [HT _]. auto.
+    split; auto.
+    destruct P1 as [_ [[v1 [Hms1 Hv1]] _]].
+    destruct P2 as [_ [[v2 [Hms2 Hv2]] _]].
+    exists (cons' v1 v2); split; auto.
+    pose proof (multistep'_cons1' _ _ (msubst' env0' t2') Hms1).
+    pose proof (multistep'_cons2' _ _ _ Hv1 Hms2).
+    apply (multi_step'_trans _ _ _ H0 H1).
+  - (* T_Case' *)
+    rewrite msubst'_case'.
+    pose proof (IHHT1 c H env0' V) as P1.
+    pose proof (IHHT2 c H env0' V) as P2.
+    clear IHHT1 IHHT2.
+    assert (WT: has_type' empty (case' (msubst' env0' t1') (msubst' env0' tnil') x y
+                  (msubst' (drop y (drop x env0')) tcons')) T').
+      { eapply T_Case';
+          try (apply R'_typable_empty; auto).
+          eapply msubst'_preserves_typing.
+          { eapply instantiation'_drop; eapply instantiation'_drop; eauto. }
+          eapply context'_invariance.
+          { apply HT3. }
+          intros.
+          unfold update, t_update. repeat rewrite mupdate'_drop.
+          destruct (eqb_spec x x0); destruct (eqb_spec y x0);
+          try auto.
+            rewrite H.
+            clear - c n n0. induction c.
+            simpl. repeat false_eqb_string; auto.
+            simpl. destruct a.  unfold update, t_update.
+            destruct (String.eqb s x0); auto. }
+    destruct (R'_halts' P1) as [v1 [Hm Hv]].
+    apply R'_typable_empty in P1 as H1, P2 as H2.
+    eapply multistep'_preserves_R1'.
+      eapply T_Case'; try assumption.
+      + inversion WT; subst. assumption.
+      + eapply multistep'_case1'. exact Hm.
+      + pose proof (canonical_forms_list' v1).
+        destruct H0.
+        eapply preservation'_multi;
+          [ exact H1 |
+            exact Hm ].
+        exact Hv.
+        * (* case nil' *)
+          clear - P2 Hm WT H0.
+          pose proof (R'_halts' P2) as [v [H1 H2]].
+          subst. eapply multistep'_preserves_R1'.
+          eapply preservation'_multi.
+          exact WT. apply multistep'_case1'. exact Hm.
+          eapply multi_step. apply ST_CaseNil'.
+          exact H1.
+          eapply multistep'_preserves_R'.
+          exact H1. exact P2.
+        * (* case cons' *)
+          clear - V P1 H H1 IHHT3 Hm WT H0.
+          destruct H0 as [v2 [v3 [Hv2 [Hv3 Heq]]]].
+          subst. eapply multistep'_preserves_R1'.
+          eapply preservation'_multi.
+          exact WT. apply multistep'_case1'. exact Hm.
+          eapply multi_step. apply ST_CaseCons'; auto.
+          apply multi_refl.
+          rewrite drop_comm.
+          apply R'_typable_empty in P1.
+          eapply (preservation'_multi) in P1; eauto.
+          inversion P1; subst; clear P1 H1.
+          repeat rewrite <- subst'_msubst';
+            eauto using typable_empty__closed',
+                        instantiation'_env'_closed'.
+          repeat rewrite msubst'_subst'.
+          apply IHHT3 with ((x,Nat')::(y,NatList')::c).
+          { intros s. unfold update, t_update, lookup.
+            destruct (eqb_spec x s); auto.
+            destruct (eqb_spec y s); auto. }
+          { repeat (constructor;
+            [auto | split; [|split];
+             auto using value'_halts' |]).
+            assumption. }
+          eapply instantiation'_env'_closed' with (drop y c).
+          apply instantiation'_drop; auto.
 Qed.
 
 Theorem normalization' : forall t' T', has_type' empty t' T' -> halts' t'.
 Proof.
   intros.
-  replace t' with (msubst' nil t') by reflexivity.
+  replace t' with (msubst' [] t') by reflexivity.
   apply (@R'_halts' T').
-  apply (msubst'_R' nil); eauto.
+  apply (msubst'_R' []); eauto.
   eapply V_nil'.
 Qed.
 
